transformations/VCGen.dfy
@@ -1,0 +1,83 @@
+
+include "../lang/Cfg.dfy"
+include "../dafny-libraries/src/Collections/Sequences/Seq.dfy"
+include "../dafny-libraries/src/Collections/Maps/Maps.dfy"
+include "../util/AstSubsetPredicates.dfy"
+include "../util/CfgHelper.dfy"
+include "../util/Util.dfy"
+
+module VCGen
+{
+
+  import opened BoogieLang
+  import opened BoogieCfg
+  import opened AstSubsetPredicates
+  import opened CfgHelper
+  import Util
+
+  function method VCBlockName(n: BlockId) : string
+  {
+    "B"+Util.NatToString(n)
+  }
+
+  function method ConjOfSuccessorVCs(bs: seq<BlockId>): Expr
+    requires |bs| >= 1
+  {
+    var vcBlock := VCBlockName(bs[0]);
+    if |bs| == 1 then
+      Var(vcBlock)
+    else
+      var expr' := ConjOfSuccessorVCs(bs[1..]);
+      BinOp(Var(vcBlock), And, expr')
+  }
+
+  function method WpSimpleCmdDeep(sc: SimpleCmd, post: Expr) : Expr
+    requires IsPassive(sc)
+  {
+    match sc
+    case Skip => post
+    case Assert(e) => BinOp(e, And, post)
+    case Assume(e) => BinOp(e, Imp, post)
+    case SeqSimple(sc1, sc2) => WpSimpleCmdDeep(sc1, WpSimpleCmdDeep(sc2, post))
+  }
+
+  function method BlockToVC(g: Cfg,  blocks: seq<BlockId>) : map<BlockId, Expr>
+    requires forall blockId | blockId in g.blocks.Keys :: IsPassive(g.blocks[blockId])
+    requires forall blockId | blockId in blocks :: blockId in g.blocks.Keys
+    ensures BlockToVC(g, blocks).Keys == (set block | block in blocks)
+  {
+    map blockId | blockId in blocks :: 
+      var successorVC :=  
+        if blockId in g.successors.Keys && |g.successors[blockId]| >= 1 then 
+          ConjOfSuccessorVCs(g.successors[blockId])
+        else
+          Expr.TrueExpr;
+      
+      WpSimpleCmdDeep(g.blocks[blockId], successorVC)
+  }
+
+  function method VCGenAux(idTopo: nat, topo: seq<BlockId>, blockMapping: map<BlockId, Expr>, result: Expr) : Expr
+    requires 0 <= idTopo <= |topo|
+    requires forall b | b in topo :: b in blockMapping.Keys
+  {
+    if idTopo == |topo| then
+      result
+    else
+      var blockId := topo[idTopo];
+      var blockVCId := VCBlockName(blockId);
+      var blockVC := blockMapping[blockId];
+      Let(blockVCId, blockVC, result)
+  }
+
+  function method VCGen(g: Cfg, topo: seq<BlockId>) : Expr
+    requires |topo| > 0
+    requires forall blockId | blockId in g.blocks.Keys :: IsPassive(g.blocks[blockId])
+    requires forall blockId | blockId in topo :: blockId in g.blocks.Keys
+  {
+    var blockToVC := BlockToVC(g, topo);
+
+    //TODO: is topo[0] the entry block?
+    VCGenAux(1, topo, blockToVC, blockToVC[topo[0]])
+  }
+
+}
